prove MakeSSA structural projection boundaries

venom/passes/make_ssa/proofs/makeSsaCurrentPropsScript.sml
@@ -1,8 +1,8 @@
 (* Structural and supply contracts for the configured MakeSSA adapter. *)
 Theory makeSsaCurrentProps
 Ancestors
-  makeSsaCurrentDefs makeSsaCurrentInduct irSupply
-  list alist
+  makeSsaCurrentDefs makeSsaCurrentInduct makeSsaHelper
+  cfgTransformProps fcgDefs irSupply list alist
 
 Definition ssa_supply_extends_def:
   ssa_supply_extends s s' <=>
@@ -177,6 +177,311 @@ Proof
      metis_tac[ssa_supply_extends_trans]
 QED
 
+
+Theorem insert_phis_for_var_supply_labels:
+  !s var df pm li bbs wl hp bbs' s'.
+    insert_phis_for_var_supply s var df pm li bbs wl hp = (bbs',s') ==>
+    MAP (\bb. bb.bb_label) bbs' = MAP (\bb. bb.bb_label) bbs
+Proof
+  recInduct insert_phis_for_var_supply_ind >>
+  rw[insert_phis_for_var_supply_def] >> gvs[]
+  >> rpt CASE_TAC >> gvs[] >> pairarg_tac >> gvs[] >>
+     drule process_frontiers_supply_labels >> strip_tac >>
+     first_x_assum drule >> simp[]
+QED
+
+Theorem add_phi_nodes_supply_labels:
+  !defs s df pm li bbs bbs' s'.
+    add_phi_nodes_supply s df pm li bbs defs = (bbs',s') ==>
+    MAP (\bb. bb.bb_label) bbs' = MAP (\bb. bb.bb_label) bbs
+Proof
+  Induct >- simp[add_phi_nodes_supply_def] >>
+  rpt gen_tac >> PairCases_on `h` >> simp[add_phi_nodes_supply_def] >>
+  pairarg_tac >> gvs[] >> strip_tac >>
+  drule insert_phis_for_var_supply_labels >> strip_tac >>
+  first_x_assum drule >> simp[]
+QED
+
+Theorem FOLDL_map_invariant:
+  !xs step acc f.
+    (!a x. MAP f (step a x) = MAP f a) ==>
+    MAP f (FOLDL step acc xs) = MAP f acc
+Proof
+  Induct >> simp[] >> rpt strip_tac >>
+  first_x_assum irule >> simp[]
+QED
+
+Theorem update_current_succ_phis_labels:
+  !succs rs current_label bbs.
+    MAP (\bb. bb.bb_label)
+      (update_current_succ_phis rs current_label bbs succs) =
+    MAP (\bb. bb.bb_label) bbs
+Proof
+  rpt gen_tac >> simp[update_current_succ_phis_def] >>
+  irule FOLDL_map_invariant >> rpt strip_tac >>
+  Cases_on `lookup_block x a` >> gvs[] >>
+  drule lookup_block_label >> strip_tac >>
+  simp[fn_labels_replace_block]
+QED
+
+Theorem rename_current_blocks_labels:
+  (!s rs bbs sm t ctrs s' bbs'.
+     rename_current_blocks s rs bbs sm t = (ctrs,s',bbs') ==>
+     MAP (\bb. bb.bb_label) bbs' = MAP (\bb. bb.bb_label) bbs) /\
+  (!s ctrs stacks bbs sm ts ctrs' s' bbs'.
+     rename_current_children s ctrs stacks bbs sm ts = (ctrs',s',bbs') ==>
+     MAP (\bb. bb.bb_label) bbs' = MAP (\bb. bb.bb_label) bbs)
+Proof
+  qsuff_tac
+    `(!t s rs bbs sm ctrs s' bbs'.
+        rename_current_blocks s rs bbs sm t = (ctrs,s',bbs') ==>
+        MAP (\bb. bb.bb_label) bbs' = MAP (\bb. bb.bb_label) bbs) /\
+     (!ts s ctrs stacks bbs sm ctrs' s' bbs'.
+        rename_current_children s ctrs stacks bbs sm ts = (ctrs',s',bbs') ==>
+        MAP (\bb. bb.bb_label) bbs' = MAP (\bb. bb.bb_label) bbs)`
+  >- metis_tac[]
+  >> ho_match_mp_tac current_dom_tree_induction >> rpt conj_tac
+  >- (rpt strip_tac >>
+      gvs[rename_current_blocks_def, AllCaseEqs()]
+      >> pairarg_tac >> gvs[] >>
+         drule lookup_block_label >> strip_tac >>
+         first_x_assum drule >> strip_tac >>
+         gvs[update_current_succ_phis_labels, fn_labels_replace_block])
+  >- simp[rename_current_blocks_def]
+  >> rpt strip_tac >> gvs[rename_current_blocks_def] >>
+     pairarg_tac >> gvs[] >>
+     first_x_assum drule >> strip_tac >>
+     first_x_assum drule >> strip_tac >>
+     metis_tac[]
+QED
+
+Theorem make_ssa_current_fn_metadata:
+  make_ssa_current_fn s fn = (fn',s') ==>
+  fn_identity_metadata_eq fn' fn /\
+  fn_static_input_eq fn' fn /\
+  fn_static_layout_eq fn' fn /\
+  fn_fmp_convention_eq fn' fn
+Proof
+  simp[make_ssa_current_fn_def] >> rpt CASE_TAC >> gvs[]
+  >- simp[venomInstTheory.fn_identity_metadata_eq_def, venomInstTheory.fn_static_input_eq_def,
+          venomInstTheory.fn_static_layout_eq_def, venomInstTheory.fn_fmp_convention_eq_def]
+  >> pairarg_tac >> gvs[] >> pairarg_tac >> gvs[] >> strip_tac >>
+     gvs[venomInstTheory.fn_identity_metadata_eq_def, venomInstTheory.fn_static_input_eq_def,
+         venomInstTheory.fn_static_layout_eq_def, venomInstTheory.fn_fmp_convention_eq_def]
+QED
+
+Theorem make_ssa_current_fn_labels:
+  make_ssa_current_fn s fn = (fn',s') ==>
+  MAP (\bb. bb.bb_label) fn'.fn_blocks =
+  MAP (\bb. bb.bb_label) fn.fn_blocks
+Proof
+  simp[make_ssa_current_fn_def] >> rpt CASE_TAC >> gvs[]
+  >> pairarg_tac >> gvs[] >> pairarg_tac >> gvs[] >> strip_tac >>
+     drule add_phi_nodes_supply_labels >> strip_tac >>
+     drule (CONJUNCT1 rename_current_blocks_labels) >> strip_tac >>
+     gvs[]
+QED
+
+Theorem make_ssa_current_fn_structural:
+  make_ssa_current_fn s fn = (fn',s') ==>
+  fn_identity_metadata_eq fn' fn /\
+  fn_static_input_eq fn' fn /\
+  fn_static_layout_eq fn' fn /\
+  fn_fmp_convention_eq fn' fn /\
+  MAP (\bb. bb.bb_label) fn'.fn_blocks =
+  MAP (\bb. bb.bb_label) fn.fn_blocks
+Proof
+  metis_tac[make_ssa_current_fn_metadata, make_ssa_current_fn_labels]
+QED
+
+Theorem rename_current_operands_label_head:
+  rename_current_operands rs (Label lbl::ops) =
+  Label lbl::rename_current_operands rs ops
+Proof
+  simp[rename_current_operands_def]
+QED
+
+Theorem rename_current_inst_invoke_target:
+  rename_current_inst s rs inst = (rs',s',inst') ==>
+  MAP FST (get_invoke_targets [inst']) =
+  MAP FST (get_invoke_targets [inst])
+Proof
+  simp[rename_current_inst_def] >> IF_CASES_TAC >> gvs[] >>
+  pairarg_tac >> gvs[] >> strip_tac >>
+  Cases_on `inst.inst_opcode = INVOKE` >> gvs[get_invoke_targets_def]
+  >- (Cases_on `inst.inst_operands` >> gvs[rename_current_operands_def] >>
+      rename1 `op::ops` >> Cases_on `op` >>
+      gvs[rename_current_operands_def])
+QED
+
+Theorem invoke_target_labels_cons:
+  MAP FST (get_invoke_targets (inst::insts)) =
+  MAP FST (get_invoke_targets [inst]) ++
+  MAP FST (get_invoke_targets insts)
+Proof
+  simp[get_invoke_targets_def] >> rpt CASE_TAC >> gvs[]
+QED
+
+Theorem rename_current_block_insts_invoke_targets:
+  !insts s rs rs' s' insts'.
+    rename_current_block_insts s rs insts = (rs',s',insts') ==>
+    MAP FST (get_invoke_targets insts') =
+    MAP FST (get_invoke_targets insts)
+Proof
+  Induct >- simp[rename_current_block_insts_def, get_invoke_targets_def] >>
+  pop_assum $ mk_asm "ih" >> rpt gen_tac >>
+  simp[rename_current_block_insts_def] >>
+  pairarg_tac >> gvs[] >> pairarg_tac >> gvs[] >> strip_tac >>
+  drule rename_current_inst_invoke_target >> strip_tac >>
+  asm "ih" drule >> strip_tac >> gvs[] >>
+  once_rewrite_tac[invoke_target_labels_cons] >> simp[]
+QED
+
+Definition block_invoke_labels_def:
+  block_invoke_labels bb =
+    MAP FST (get_invoke_targets bb.bb_instructions)
+End
+
+
+Theorem MAP_if_not_mem:
+  !xs p (y:'a).
+    (!x. MEM x xs ==> ~p x) ==>
+    MAP (\x. if p x then y else x) xs = xs
+Proof
+  Induct >> simp[] >> metis_tac[]
+QED
+
+Theorem MAP_replace_at_FIND_distinct:
+  !xs (key:'a -> 'b) k old new (f:'a -> 'c).
+    ALL_DISTINCT (MAP key xs) /\
+    FIND (\x. key x = k) xs = SOME old /\
+    f new = f old ==>
+    MAP f (MAP (\x. if key x = k then new else x) xs) = MAP f xs
+Proof
+  Induct >- simp[] >> rpt gen_tac >>
+  simp[listTheory.FIND_thm] >> rpt strip_tac >>
+  Cases_on `key h = k`
+  >- (gvs[MEM_MAP] >>
+      `MAP (\x. if key x = k then new else x) xs = xs` by
+        (ho_match_mp_tac MAP_if_not_mem >> metis_tac[]) >>
+      simp[])
+  >> gvs[MEM_MAP] >>
+  `MAP (\x. if key x = key h then new else x) xs = xs` by
+    (ho_match_mp_tac MAP_if_not_mem >> rpt strip_tac >>
+     qpat_x_assum `!y. key h = key y ==> ~MEM y xs`
+       (qspec_then `x` mp_tac) >> simp[]) >>
+  simp[]
+QED
+
+Theorem bb_label_eta:
+  (\bb. bb.bb_label) = basic_block_bb_label
+Proof
+  simp[FUN_EQ_THM]
+QED
+
+Theorem replace_block_invoke_labels_distinct:
+  !bbs lbl bb bb'.
+    ALL_DISTINCT (MAP basic_block_bb_label bbs) /\
+    lookup_block lbl bbs = SOME bb /\
+    bb'.bb_label = lbl /\
+    block_invoke_labels bb' = block_invoke_labels bb ==>
+    MAP block_invoke_labels (replace_block lbl bb' bbs) =
+    MAP block_invoke_labels bbs
+Proof
+  rpt strip_tac >>
+  simp[cfgTransformTheory.replace_block_def] >>
+  ho_match_mp_tac MAP_replace_at_FIND_distinct >>
+  qexists `bb` >> conj_tac
+  >- (qpat_assum `ALL_DISTINCT _` mp_tac >> simp[GSYM bb_label_eta])
+  >> gvs[venomInstTheory.lookup_block_def]
+QED
+
+Theorem invoke_target_labels_append:
+  !xs ys.
+    MAP FST (get_invoke_targets (xs ++ ys)) =
+    MAP FST (get_invoke_targets xs) ++ MAP FST (get_invoke_targets ys)
+Proof
+  Induct >- simp[get_invoke_targets_def] >> rpt gen_tac >>
+  pure_once_rewrite_tac[APPEND] >>
+  once_rewrite_tac[invoke_target_labels_cons] >> simp[]
+QED
+
+Theorem fn_insts_blocks_invoke_labels:
+  !bbs.
+    MAP FST (get_invoke_targets (fn_insts_blocks bbs)) =
+    FLAT (MAP block_invoke_labels bbs)
+Proof
+  Induct >>
+  simp[venomInstTheory.fn_insts_blocks_def, block_invoke_labels_def,
+       invoke_target_labels_append, get_invoke_targets_def]
+QED
+
+Theorem fcg_scan_function_invoke_labels:
+  MAP FST (fcg_scan_function fn) =
+  FLAT (MAP block_invoke_labels fn.fn_blocks)
+Proof
+  simp[fcg_scan_function_def, venomInstTheory.fn_insts_def,
+       fn_insts_blocks_invoke_labels]
+QED
+
+Theorem insert_phi_at_block_invoke_labels:
+  phi.inst_opcode = PHI ==>
+  block_invoke_labels (insert_phi_at_block phi bb) = block_invoke_labels bb
+Proof
+  simp[block_invoke_labels_def, makeSsaDefsTheory.insert_phi_at_block_def,
+       get_invoke_targets_def]
+QED
+
+
+Theorem process_frontiers_supply_invoke_labels:
+  !fs s var pm li bbs rest hp bbs' rest' hp' s'.
+    process_frontiers_supply s var pm li bbs rest hp fs =
+      (bbs',rest',hp',s') ==>
+    MAP block_invoke_labels bbs' = MAP block_invoke_labels bbs
+Proof
+  Induct >- simp[process_frontiers_supply_def] >>
+  pop_assum $ mk_asm "ih" >>
+  simp[process_frontiers_supply_def] >> rpt gen_tac >>
+  IF_CASES_TAC >> gvs[]
+  >- (strip_tac >> asm "ih" drule >> simp[])
+  >> IF_CASES_TAC >> gvs[]
+  >- (strip_tac >> asm "ih" drule >> simp[])
+  >> rpt CASE_TAC >> gvs[] >> pairarg_tac >> gvs[] >> strip_tac >>
+  asm "ih" drule >> rw[MAP_MAP_o] >>
+  irule MAP_CONG >> rw[] >>
+  Cases_on `e.bb_label = h` >>
+  simp[makeSsaDefsTheory.insert_phi_at_block_def,
+       block_invoke_labels_def, build_phi_inst_supply_def,
+       get_invoke_targets_def]
+QED
+
+
+
+Theorem insert_phis_for_var_supply_invoke_labels:
+  !s var df pm li bbs wl hp bbs' s'.
+    insert_phis_for_var_supply s var df pm li bbs wl hp = (bbs',s') ==>
+    MAP block_invoke_labels bbs' = MAP block_invoke_labels bbs
+Proof
+  recInduct insert_phis_for_var_supply_ind >>
+  rw[insert_phis_for_var_supply_def] >> gvs[] >>
+  rpt CASE_TAC >> gvs[] >> pairarg_tac >> gvs[] >>
+  drule process_frontiers_supply_invoke_labels >> strip_tac >>
+  first_x_assum drule >> simp[]
+QED
+
+Theorem add_phi_nodes_supply_invoke_labels:
+  !defs s df pm li bbs bbs' s'.
+    add_phi_nodes_supply s df pm li bbs defs = (bbs',s') ==>
+    MAP block_invoke_labels bbs' = MAP block_invoke_labels bbs
+Proof
+  Induct >- simp[add_phi_nodes_supply_def] >>
+  rpt gen_tac >> PairCases_on `h` >> simp[add_phi_nodes_supply_def] >>
+  pairarg_tac >> gvs[] >> strip_tac >>
+  drule insert_phis_for_var_supply_invoke_labels >> strip_tac >>
+  first_x_assum drule >> simp[]
+QED
+
+
 Theorem make_ssa_functions_supply_extends:
   !fns s fns' s'.
     make_ssa_functions_supply s fns = (fns',s') ==>
@@ -203,6 +508,21 @@ Theorem make_ssa_unit_supply_extends:
 Proof
   simp[make_ssa_unit_supply_def] >> pairarg_tac >> gvs[] >> strip_tac >>
   drule make_ssa_ctx_supply_extends >> simp[]
+QED
+
+
+Theorem make_ssa_current_fn_duplicate_label_invoke_probe:
+  let s = <| irs_next_inst := 1; irs_next_var := 0; irs_next_label := 0;
+             irs_used_inst_ids := [0]; irs_used_vars := [];
+             irs_used_labels := ["entry"] |> in
+  let invoke = mk_inst 0 INVOKE [Label "callee"] [] in
+  let bb0 = <| bb_label := "entry"; bb_instructions := [] |> in
+  let bb1 = <| bb_label := "entry"; bb_instructions := [invoke] |> in
+  let fn = mk_raw_function "f" [bb0;bb1] in
+    MAP FST (fcg_scan_function (FST (make_ssa_current_fn s fn))) <>
+    MAP FST (fcg_scan_function fn)
+Proof
+  EVAL_TAC
 QED
 
 val _ = export_theory();
